rename consistentM -> cmem, consistentS -> crel_vs, consistentPred -> cpred_s

DP_Consistency.thy
@@ -11,216 +11,216 @@ context
 begin
   
   (* Predicates *)
-definition consistentM :: "('param \<rightharpoonup> 'result) \<Rightarrow> bool" where
-  "consistentM M \<equiv> \<forall>param\<in>dom M. M param = Some (dp param)"
+definition cmem :: "('param \<rightharpoonup> 'result) \<Rightarrow> bool" where
+  "cmem M \<equiv> \<forall>param\<in>dom M. M param = Some (dp param)"
 term 0 (**)
   
-definition consistentS :: "('a \<Rightarrow> 'b \<Rightarrow> bool) \<Rightarrow> 'a \<Rightarrow> ('param \<rightharpoonup> 'result, 'b) state \<Rightarrow> bool" where
-  "consistentS R v s \<equiv> \<forall>M. consistentM M \<longrightarrow> (case runState s M of (v', M') \<Rightarrow> R v v' \<and> consistentM M')"
+definition crel_vs :: "('a \<Rightarrow> 'b \<Rightarrow> bool) \<Rightarrow> 'a \<Rightarrow> ('param \<rightharpoonup> 'result, 'b) state \<Rightarrow> bool" where
+  "crel_vs R v s \<equiv> \<forall>M. cmem M \<longrightarrow> (case runState s M of (v', M') \<Rightarrow> R v v' \<and> cmem M')"
   
-definition consistentS_alt :: "('a \<Rightarrow> 'b \<Rightarrow> bool) \<Rightarrow> 'a \<Rightarrow> ('param \<rightharpoonup> 'result, 'b) state \<Rightarrow> bool" where
-  "consistentS_alt R v s \<equiv> pred_fun consistentM (pred_prod (R v) consistentM) (runState s)"
+definition crel_vs_alt :: "('a \<Rightarrow> 'b \<Rightarrow> bool) \<Rightarrow> 'a \<Rightarrow> ('param \<rightharpoonup> 'result, 'b) state \<Rightarrow> bool" where
+  "crel_vs_alt R v s \<equiv> pred_fun cmem (pred_prod (R v) cmem) (runState s)"
 
-lemma "consistentS = consistentS_alt"
-  unfolding consistentS_def consistentS_alt_def
+abbreviation rel_fun_lifted :: "('a \<Rightarrow> 'c \<Rightarrow> bool) \<Rightarrow> ('b \<Rightarrow> 'd \<Rightarrow> bool) \<Rightarrow> ('a \<Rightarrow> 'b) \<Rightarrow> ('c ==_\<Longrightarrow> 'd) \<Rightarrow> bool" (infixr "===>\<^sub>T" 55) where
+  "rel_fun_lifted R R' \<equiv> R ===> crel_vs R'"
+term 0 (**)
+
+lemma "crel_vs = crel_vs_alt"
+  unfolding crel_vs_def crel_vs_alt_def
   by (fastforce split: pred_prod_split)
 term 0 (**)
   
-abbreviation rel_fun_lifted :: "('a \<Rightarrow> 'c \<Rightarrow> bool) \<Rightarrow> ('b \<Rightarrow> 'd \<Rightarrow> bool) \<Rightarrow> ('a \<Rightarrow> 'b) \<Rightarrow> ('c ==_\<Longrightarrow> 'd) \<Rightarrow> bool" (infixr "===>\<^sub>T" 55) where
-  "A ===>\<^sub>T B \<equiv> A ===> consistentS B"
-term 0 (**)
-  
 definition consistentDP :: "('param \<Rightarrow>\<^sub>T 'result) \<Rightarrow> bool" where
-  "consistentDP \<equiv> (op = ===>\<^sub>T op =) dp"
+  "consistentDP \<equiv> (op = ===> crel_vs op =) dp"
 term 0 (**)
   
-  (* consistentM *)
-lemma consistentM_intro:
+  (* cmem *)
+lemma cmem_intro:
   assumes "\<And>param v. M param = Some v \<Longrightarrow> v = dp param"
-  shows "consistentM M"
-  using assms unfolding consistentM_def by blast
+  shows "cmem M"
+  using assms unfolding cmem_def by blast
 term 0 (**)
   
-lemma consistentM_elim:
-  assumes "consistentM M" "M param = Some v"
+lemma cmem_elim:
+  assumes "cmem M" "M param = Some v"
   obtains "dp param = v"
-  using assms unfolding consistentM_def dom_def by auto
+  using assms unfolding cmem_def dom_def by auto
 term 0 (**)
   
-  (* consistentS *)
-lemma consistentS_intro:
-  assumes "\<And>M v' M'. \<lbrakk>consistentM M; runState v\<^sub>T M = (v', M')\<rbrakk> \<Longrightarrow> R v v' \<and> consistentM M'"
-  shows "consistentS R v v\<^sub>T"
-  using assms unfolding consistentS_def by blast
+  (* crel_vs *)
+lemma crel_vs_intro:
+  assumes "\<And>M v' M'. \<lbrakk>cmem M; runState v\<^sub>T M = (v', M')\<rbrakk> \<Longrightarrow> R v v' \<and> cmem M'"
+  shows "crel_vs R v v\<^sub>T"
+  using assms unfolding crel_vs_def by blast
 term 0 (**)
   
-lemma consistentS_elim:
-  assumes "consistentS R v v\<^sub>T" "consistentM M"
-  obtains v' M' where "runState v\<^sub>T M = (v', M')" "R v v'" "consistentM M'"
-  using assms unfolding consistentS_def by blast
+lemma crel_vs_elim:
+  assumes "crel_vs R v v\<^sub>T" "cmem M"
+  obtains v' M' where "runState v\<^sub>T M = (v', M')" "R v v'" "cmem M'"
+  using assms unfolding crel_vs_def by blast
 term 0 (**)
   
   (* consistentDP *)
 lemma consistentDP_intro:
-  assumes "\<And>param. consistentS (op =) (dp param) (dp\<^sub>T param)"
+  assumes "\<And>param. crel_vs (op =) (dp param) (dp\<^sub>T param)"
   shows "consistentDP dp\<^sub>T"
   using assms unfolding consistentDP_def by blast
 term 0 (**)
   
-lemma consistentS_return:
-  "\<lbrakk>R x y\<rbrakk> \<Longrightarrow> consistentS R x (return y)"
-  unfolding return_def by (fastforce intro: consistentS_intro)
+lemma crel_vs_return:
+  "\<lbrakk>R x y\<rbrakk> \<Longrightarrow> crel_vs R x (return y)"
+  unfolding return_def by (fastforce intro: crel_vs_intro)
 term 0 (**)
   
   (* Low level operators *)
-lemma consistentM_upd:
-  "\<lbrakk>consistentM M; v = dp param\<rbrakk> \<Longrightarrow> consistentM (M(param\<mapsto>v))"
-  unfolding consistentM_def by auto
+lemma cmem_upd:
+  "\<lbrakk>cmem M; v = dp param\<rbrakk> \<Longrightarrow> cmem (M(param\<mapsto>v))"
+  unfolding cmem_def by auto
 term 0 (**)
   
-lemma consistentS_get:
-  "\<lbrakk>\<And>M. consistentM M \<Longrightarrow> consistentS R v (sf M)\<rbrakk> \<Longrightarrow> consistentS R v (get \<bind> sf)"
-  unfolding get_def bind_def by (fastforce intro: consistentS_intro elim: consistentS_elim split: prod.split)
+lemma crel_vs_get:
+  "\<lbrakk>\<And>M. cmem M \<Longrightarrow> crel_vs R v (sf M)\<rbrakk> \<Longrightarrow> crel_vs R v (get \<bind> sf)"
+  unfolding get_def bind_def by (fastforce intro: crel_vs_intro elim: crel_vs_elim split: prod.split)
 term 0 (**)
   
-lemma consistentS_put:
-  "\<lbrakk>consistentS R v sf; consistentM M\<rbrakk> \<Longrightarrow> consistentS R v (put M \<then> sf)"
-  unfolding put_def bind_def by (fastforce intro: consistentS_intro elim: consistentS_elim split: prod.split)
+lemma crel_vs_put:
+  "\<lbrakk>crel_vs R v sf; cmem M\<rbrakk> \<Longrightarrow> crel_vs R v (put M \<then> sf)"
+  unfolding put_def bind_def by (fastforce intro: crel_vs_intro elim: crel_vs_elim split: prod.split)
 term 0 (**)
   
-lemma consistentS_bind_eq:
-  "\<lbrakk>consistentS op = v s; consistentS R (f v) (sf v)\<rbrakk> \<Longrightarrow> consistentS R (f v) (s \<bind> sf)"
-  unfolding bind_def rel_fun_def by (fastforce intro: consistentS_intro elim: consistentS_elim split: prod.split)
+lemma crel_vs_bind_eq:
+  "\<lbrakk>crel_vs op = v s; crel_vs R (f v) (sf v)\<rbrakk> \<Longrightarrow> crel_vs R (f v) (s \<bind> sf)"
+  unfolding bind_def rel_fun_def by (fastforce intro: crel_vs_intro elim: crel_vs_elim split: prod.split)
 term 0 (**)
   
-lemma consistentS_checkmem:
-  "\<lbrakk>consistentS op = (dp param) s\<rbrakk> \<Longrightarrow> consistentS op = (dp param) (checkmem param s)"
-  unfolding checkmem_def by (fastforce intro: consistentS_return consistentS_get consistentS_put
-      consistentS_bind_eq consistentM_upd elim: consistentM_elim split: option.splits)
+lemma crel_vs_checkmem:
+  "\<lbrakk>crel_vs op = (dp param) s\<rbrakk> \<Longrightarrow> crel_vs op = (dp param) (checkmem param s)"
+  unfolding checkmem_def by (fastforce intro: crel_vs_return crel_vs_get crel_vs_put
+      crel_vs_bind_eq cmem_upd elim: cmem_elim split: option.splits)
 term 0 (**)
   
   (** Transfer rules **)
   (* Basics *)
 lemma return_transfer[transfer_rule]:
   "(R ===>\<^sub>T R) (\<lambda>x. x) return"
-  unfolding id_def rel_fun_def by (metis consistentS_return)
+  unfolding id_def rel_fun_def by (metis crel_vs_return)
     
 lemma bind_transfer[transfer_rule]:
-  "(consistentS R0 ===> (R0 ===>\<^sub>T R1) ===> consistentS R1) (\<lambda>v f. f v) (op \<bind>)"
-  unfolding bind_def rel_fun_def by (fastforce intro: consistentS_intro elim: consistentS_elim split: prod.split)
+  "(crel_vs R0 ===> (R0 ===>\<^sub>T R1) ===> crel_vs R1) (\<lambda>v f. f v) (op \<bind>)"
+  unfolding bind_def rel_fun_def by (fastforce intro: crel_vs_intro elim: crel_vs_elim split: prod.split)
     
 lemma fun_app_lifted_transfer[transfer_rule]:
-  "(consistentS (R0 ===>\<^sub>T R1) ===> consistentS R0 ===> consistentS R1) (\<lambda> f x. f x) (op .)"
+  "(crel_vs (R0 ===>\<^sub>T R1) ===> crel_vs R0 ===> crel_vs R1) (\<lambda> f x. f x) (op .)"
   unfolding fun_app_lifted_def by transfer_prover
 
 term 0 (**)
 
 lemma unlift_'_transfer[transfer_rule]:
-  "(R ===> consistentS R) (\<lambda> x. x) unlift_'"
+  "(R ===> crel_vs R) (\<lambda> x. x) unlift_'"
   unfolding unlift_'_def by transfer_prover
 term 0 (**)
   
 lemma unlift_3_transfer[transfer_rule]:
-  "((R0 ===>\<^sub>T R1) ===> (R0 ===> consistentS R1)) (\<lambda> f x. f x) unlift_3"
+  "((R0 ===>\<^sub>T R1) ===> (R0 ===> crel_vs R1)) (\<lambda> f x. f x) unlift_3"
   unfolding unlift_3_def by transfer_prover
 term 0 (**)
   
 lemma unlift_33_transfer[transfer_rule]:
-  "((R0 ===>\<^sub>T R1 ===>\<^sub>T R2) ===> (R0 ===> R1 ===> consistentS R2)) (\<lambda> f x0 x1. f x0 x1) unlift_33"
+  "((R0 ===>\<^sub>T R1 ===>\<^sub>T R2) ===> (R0 ===> R1 ===> crel_vs R2)) (\<lambda> f x0 x1. f x0 x1) unlift_33"
   unfolding unlift_33_def by transfer_prover
 
 lemma lift_'_transfer[transfer_rule]:
-  "(R ===> consistentS R) (\<lambda> x. x) lift_'"
+  "(R ===> crel_vs R) (\<lambda> x. x) lift_'"
   unfolding lift_'_def by transfer_prover
 
 lemma lift_3_transfer[transfer_rule]:
-  "((R0 ===> R1) ===> consistentS (R0 ===>\<^sub>T R1)) (\<lambda> f x. f x) lift_3"
+  "((R0 ===> R1) ===> crel_vs (R0 ===>\<^sub>T R1)) (\<lambda> f x. f x) lift_3"
   unfolding lift_3_def by transfer_prover
     
 lemma lift_33_transfer[transfer_rule]:
-  "((R0 ===> R1 ===> R2) ===> consistentS (R0 ===>\<^sub>T R1 ===>\<^sub>T R2)) (\<lambda> f x0 x1. f x0 x1) lift_33"
+  "((R0 ===> R1 ===> R2) ===> crel_vs (R0 ===>\<^sub>T R1 ===>\<^sub>T R2)) (\<lambda> f x0 x1. f x0 x1) lift_33"
   unfolding lift_33_def by transfer_prover
 
 lemma lift_333_transfer[transfer_rule]:
-  "((R0 ===> R1 ===> R2 ===> R3) ===> consistentS (R0 ===>\<^sub>T R1 ===>\<^sub>T R2 ===>\<^sub>T R3)) (\<lambda> f x0 x1 x2. f x0 x1 x2) lift_333"
+  "((R0 ===> R1 ===> R2 ===> R3) ===> crel_vs (R0 ===>\<^sub>T R1 ===>\<^sub>T R2 ===>\<^sub>T R3)) (\<lambda> f x0 x1 x2. f x0 x1 x2) lift_333"
   unfolding lift_333_def by transfer_prover
 term 0 (**)
 
   (* HOL *)
 lemma If_transfer[transfer_rule]:
-  "consistentS (op = ===>\<^sub>T R ===>\<^sub>T R ===>\<^sub>T R) If If\<^sub>T"
+  "crel_vs (op = ===>\<^sub>T R ===>\<^sub>T R ===>\<^sub>T R) If If\<^sub>T"
   unfolding If\<^sub>T_def by transfer_prover
   
 lemma id_transfer[transfer_rule]:
-  "consistentS (R ===>\<^sub>T R) id id\<^sub>T"
+  "crel_vs (R ===>\<^sub>T R) id id\<^sub>T"
   unfolding id_def id\<^sub>T_def by transfer_prover
     
 lemma comp_transfer[transfer_rule]:
-  "consistentS ((R1 ===>\<^sub>T R2) ===>\<^sub>T (R0 ===>\<^sub>T R1) ===>\<^sub>T (R0 ===>\<^sub>T R2)) comp comp\<^sub>T"
+  "crel_vs ((R1 ===>\<^sub>T R2) ===>\<^sub>T (R0 ===>\<^sub>T R1) ===>\<^sub>T (R0 ===>\<^sub>T R2)) comp comp\<^sub>T"
   unfolding comp_def comp\<^sub>T_def fun_app_lifted_def by transfer_prover
 term 0 (**)
 
   (* Arithmetic *)
 
 lemma plus_transfer[transfer_rule]:
-  "consistentS (op = ===>\<^sub>T op = ===>\<^sub>T op =) plus plus\<^sub>T"
+  "crel_vs (op = ===>\<^sub>T op = ===>\<^sub>T op =) plus plus\<^sub>T"
   unfolding plus\<^sub>T_def by transfer_prover
   
 lemma min_transfer[transfer_rule]:
-  "consistentS (op = ===>\<^sub>T op = ===>\<^sub>T op =) min min\<^sub>T"
+  "crel_vs (op = ===>\<^sub>T op = ===>\<^sub>T op =) min min\<^sub>T"
   unfolding min\<^sub>T_def by transfer_prover
     
 lemma max_transfer[transfer_rule]:
-  "consistentS (op = ===>\<^sub>T op = ===>\<^sub>T op =) max max\<^sub>T"
+  "crel_vs (op = ===>\<^sub>T op = ===>\<^sub>T op =) max max\<^sub>T"
   unfolding max\<^sub>T_def by transfer_prover
 term 0 (**)  
 
   (* Option *)
 lemma case_option_transfer[transfer_rule]:
-  "consistentS (R1 ===>\<^sub>T (R0 ===>\<^sub>T R1) ===>\<^sub>T rel_option R0 ===>\<^sub>T R1) case_option case_option\<^sub>T"
+  "crel_vs (R1 ===>\<^sub>T (R0 ===>\<^sub>T R1) ===>\<^sub>T rel_option R0 ===>\<^sub>T R1) case_option case_option\<^sub>T"
   unfolding case_option\<^sub>T_def by transfer_prover
 
 lemma None_transfer[transfer_rule]:
-  "consistentS (rel_option R) None None\<^sub>T"
+  "crel_vs (rel_option R) None None\<^sub>T"
   unfolding None\<^sub>T_def by transfer_prover
 
 lemma Some_transfer[transfer_rule]:
-  "consistentS (R ===>\<^sub>T rel_option R) Some Some\<^sub>T"
+  "crel_vs (R ===>\<^sub>T rel_option R) Some Some\<^sub>T"
   unfolding Some\<^sub>T_def by transfer_prover
 term 0 (**)
 
   (* List *)  
 lemma case_list_transfer[transfer_rule]:
-  "consistentS (R1 ===>\<^sub>T (R0 ===>\<^sub>T list_all2 R0 ===>\<^sub>T R1) ===>\<^sub>T list_all2 R0 ===>\<^sub>T R1) case_list case_list\<^sub>T"
+  "crel_vs (R1 ===>\<^sub>T (R0 ===>\<^sub>T list_all2 R0 ===>\<^sub>T R1) ===>\<^sub>T list_all2 R0 ===>\<^sub>T R1) case_list case_list\<^sub>T"
   unfolding case_list\<^sub>T_def by transfer_prover
   
 lemma Nil_transfer[transfer_rule]:
-  "consistentS (list_all2 R) Nil Nil\<^sub>T"
+  "crel_vs (list_all2 R) Nil Nil\<^sub>T"
   unfolding Nil\<^sub>T_def by transfer_prover
 
 lemma Cons_transfer[transfer_rule]:
-  "consistentS (R ===>\<^sub>T list_all2 R ===>\<^sub>T list_all2 R) Cons Cons\<^sub>T"
+  "crel_vs (R ===>\<^sub>T list_all2 R ===>\<^sub>T list_all2 R) Cons Cons\<^sub>T"
   unfolding Cons\<^sub>T_def by transfer_prover
     
 lemma upt_transfer[transfer_rule]:
-  "consistentS (op = ===>\<^sub>T op = ===>\<^sub>T list_all2 op =) upt upt\<^sub>T"
+  "crel_vs (op = ===>\<^sub>T op = ===>\<^sub>T list_all2 op =) upt upt\<^sub>T"
   unfolding upt\<^sub>T_def by transfer_prover
 term 0 (**)
   
   (* Prod *)
 lemma case_prod_transfer[transfer_rule]:
-  "consistentS ((R0 ===>\<^sub>T R1 ===>\<^sub>T R2) ===>\<^sub>T rel_prod R0 R1 ===>\<^sub>T R2) case_prod case_prod\<^sub>T"
+  "crel_vs ((R0 ===>\<^sub>T R1 ===>\<^sub>T R2) ===>\<^sub>T rel_prod R0 R1 ===>\<^sub>T R2) case_prod case_prod\<^sub>T"
   unfolding case_prod\<^sub>T_def by transfer_prover
 term 0 (**)
   
 lemma Pair_transfer[transfer_rule]:
-  "consistentS (R0 ===>\<^sub>T R1 ===>\<^sub>T rel_prod R0 R1) Pair Pair\<^sub>T"
+  "crel_vs (R0 ===>\<^sub>T R1 ===>\<^sub>T rel_prod R0 R1) Pair Pair\<^sub>T"
   unfolding Pair\<^sub>T_def by transfer_prover
 term 0 (**)
 
   (* Combinator *)
 lemma map_transfer[transfer_rule]:
-  "consistentS ((R0 ===>\<^sub>T R1) ===>\<^sub>T list_all2 R0 ===>\<^sub>T list_all2 R1) map map\<^sub>T"
+  "crel_vs ((R0 ===>\<^sub>T R1) ===>\<^sub>T list_all2 R0 ===>\<^sub>T list_all2 R1) map map\<^sub>T"
 proof -
   have [transfer_rule]: "((R0 ===>\<^sub>T R1) ===> (list_all2 R0 ===>\<^sub>T list_all2 R1)) map map\<^sub>T'"
     apply ((rule rel_funI)+, induct_tac rule: list_all2_induct, assumption; unfold list.map map\<^sub>T'.simps)
@@ -232,7 +232,7 @@ proof -
 qed
   
 lemma fold_transfer[transfer_rule]:
-  "consistentS ((R0 ===>\<^sub>T R1 ===>\<^sub>T R1) ===>\<^sub>T list_all2 R0 ===>\<^sub>T R1 ===>\<^sub>T R1) fold fold\<^sub>T"
+  "crel_vs ((R0 ===>\<^sub>T R1 ===>\<^sub>T R1) ===>\<^sub>T list_all2 R0 ===>\<^sub>T R1 ===>\<^sub>T R1) fold fold\<^sub>T"
 proof -
   have [transfer_rule]: "((R0 ===>\<^sub>T R1 ===>\<^sub>T R1) ===> list_all2 R0 ===>\<^sub>T R1 ===>\<^sub>T R1) fold fold\<^sub>T'"
     apply ((rule rel_funI)+, induct_tac rule: list_all2_induct, assumption; unfold fold.simps fold\<^sub>T'.simps)
