DP_Pred.thy
@@ -7,48 +7,48 @@ context
   includes lifting_syntax
 begin
   
-definition consistentPred :: "('a \<Rightarrow> bool) \<Rightarrow> ('param \<rightharpoonup> 'result, 'a) state \<Rightarrow> bool" where
-  "consistentPred P s \<equiv> \<forall>M. consistentM M \<longrightarrow> (case runState s M of (v', M') \<Rightarrow> P v' \<and> consistentM M')"
+definition cpred_s :: "('a \<Rightarrow> bool) \<Rightarrow> ('param \<rightharpoonup> 'result, 'a) state \<Rightarrow> bool" where
+  "cpred_s P s \<equiv> \<forall>M. cmem M \<longrightarrow> (case runState s M of (v', M') \<Rightarrow> P v' \<and> cmem M')"
   
-definition consistentPred_alt :: "('a \<Rightarrow> bool) \<Rightarrow> ('param \<rightharpoonup> 'result, 'a) state \<Rightarrow> bool" where
-  "consistentPred_alt P s \<equiv> pred_fun consistentM (pred_prod P consistentM) (runState s)"
+definition cpred_s_alt :: "('a \<Rightarrow> bool) \<Rightarrow> ('param \<rightharpoonup> 'result, 'a) state \<Rightarrow> bool" where
+  "cpred_s_alt P s \<equiv> pred_fun cmem (pred_prod P cmem) (runState s)"
   
-lemma "consistentPred_alt = consistentPred"
-  unfolding consistentPred_def consistentPred_alt_def
+lemma "cpred_s_alt = cpred_s"
+  unfolding cpred_s_def cpred_s_alt_def
   by (fastforce split: pred_prod_split)
 term 0(**)
 
 notation pred_fun (infixr "...>" 55)
 
 abbreviation pred_fun_lifted :: "('a \<Rightarrow> bool) \<Rightarrow> ('b \<Rightarrow> bool) \<Rightarrow> ('a ==_\<Longrightarrow> 'b) \<Rightarrow> bool" (infixr "...>\<^sub>T" 55) where
-  "A ...>\<^sub>T B \<equiv> A ...> consistentPred B"
+  "A ...>\<^sub>T B \<equiv> A ...> cpred_s B"
 
   
-lemma consistentPred_intro:
-  assumes "\<And>M v' M'. \<lbrakk>consistentM M; runState v\<^sub>T M = (v', M')\<rbrakk> \<Longrightarrow> P v' \<and> consistentM M'"
-  shows "consistentPred P v\<^sub>T"
-  unfolding consistentPred_def using assms by blast
+lemma cpred_s_intro:
+  assumes "\<And>M v' M'. \<lbrakk>cmem M; runState v\<^sub>T M = (v', M')\<rbrakk> \<Longrightarrow> P v' \<and> cmem M'"
+  shows "cpred_s P v\<^sub>T"
+  unfolding cpred_s_def using assms by blast
 
-lemma consistentPred_elim:
-  assumes "consistentPred P v\<^sub>T" "consistentM M"
-  obtains v' M' where "runState v\<^sub>T M = (v', M')" "P v'" "consistentM M'"
-  using assms unfolding consistentPred_def by blast
+lemma cpred_s_elim:
+  assumes "cpred_s P v\<^sub>T" "cmem M"
+  obtains v' M' where "runState v\<^sub>T M = (v', M')" "P v'" "cmem M'"
+  using assms unfolding cpred_s_def by blast
 term 0 (**)
 
-lemma consistentPred_return:
-  "P v \<Longrightarrow> consistentPred P \<langle>v\<rangle>"
-  unfolding return_def by (fastforce intro: consistentPred_intro)
+lemma cpred_s_return:
+  "P v \<Longrightarrow> cpred_s P \<langle>v\<rangle>"
+  unfolding return_def by (fastforce intro: cpred_s_intro)
 
 lemma return_transferP:
-  "(P ...> consistentPred P) return"
-  unfolding pred_fun_def by (metis consistentPred_return)
+  "(P ...> cpred_s P) return"
+  unfolding pred_fun_def by (metis cpred_s_return)
     
 lemma bind_transferP:
-  "(consistentPred P0 ...> (P0 ...>\<^sub>T P1) ...> consistentPred P1) (op \<bind>)"
-  unfolding bind_def pred_fun_def by (fastforce intro: consistentPred_intro elim: consistentPred_elim split: prod.split)
+  "(cpred_s P0 ...> (P0 ...>\<^sub>T P1) ...> cpred_s P1) (op \<bind>)"
+  unfolding bind_def pred_fun_def by (fastforce intro: cpred_s_intro elim: cpred_s_elim split: prod.split)
     
 lemma fun_app_lifted_transferP:
-  "(consistentPred (R0 ...>\<^sub>T R1) ...> consistentPred P0 ...> consistentPred P1) (op .)"
+  "(cpred_s (R0 ...>\<^sub>T R1) ...> cpred_s P0 ...> cpred_s P1) (op .)"
   unfolding fun_app_lifted_def
   oops 
 end
