example/Bellman_Ford.thy
@@ -23,6 +23,14 @@ fun bf :: "nat\<times>nat \<Rightarrow> int" where
           (upt 0 n))
       (bf (k, j))"
 thm bf.simps
+thm bf.induct
+term 0 (**)
+  
+lemma map\<^sub>T_return_return_cong[fundef_cong]:
+  fixes f g xs
+  assumes "\<And>x. x\<in>set xs \<Longrightarrow> f x = g x"
+  shows "map\<^sub>T . \<langle>f\<rangle> . \<langle>xs\<rangle> = map\<^sub>T . \<langle>g\<rangle> . \<langle>xs\<rangle>"
+  sorry
 term 0 (**)
   
 fun bf\<^sub>T :: "nat\<times>nat \<Rightarrow>\<^sub>T int" where
@@ -32,8 +40,10 @@ fun bf\<^sub>T :: "nat\<times>nat \<Rightarrow>\<^sub>T int" where
     . min\<^sub>T
     . (map\<^sub>T
       . (\<lambda>\<^sub>Ti. plus\<^sub>T . \<langle>W i j\<rangle> . (bf\<^sub>T (k, i)))
-      . (upt\<^sub>T . \<langle>0\<rangle> . \<langle>n\<rangle>))
+      . \<langle>upt 0 n\<rangle>)
     . (bf\<^sub>T (k, j))"
+thm bf\<^sub>T.simps
+thm bf\<^sub>T.induct
 term 0 (**)
   
 interpretation bf: dp_consistency bf .
@@ -47,7 +57,7 @@ term 0 (**)
 
 lemma bf_induct:
   "\<lbrakk>\<And>j. P (0, j);
-    \<And>k j. \<lbrakk>\<And>x. P (k, x);
+    \<And>k j. \<lbrakk>\<And>x. x \<in> set [0..<n] \<Longrightarrow> P (k, x);
            P (k, j)
            \<rbrakk> \<Longrightarrow> P (Suc k, j)
    \<rbrakk> \<Longrightarrow> P (x::nat\<times>nat)"
@@ -55,7 +65,7 @@ lemma bf_induct:
 
 lemma bf_inductS:
   "\<lbrakk>\<And>j. bf.consistentS op = (bf (0, j)) (bf\<^sub>T (0, j));
-    \<And>k j. \<lbrakk>\<And>x. bf.consistentS op = (bf (k, x)) (bf\<^sub>T (k, x));
+    \<And>k j. \<lbrakk>\<And>x. x \<in> set [0..<n] \<Longrightarrow> bf.consistentS op = (bf (k, x)) (bf\<^sub>T (k, x));
            bf.consistentS op = (bf (k, j)) (bf\<^sub>T (k, j))
            \<rbrakk> \<Longrightarrow> bf.consistentS op = (bf (Suc k, j)) (bf\<^sub>T (Suc k, j))
    \<rbrakk> \<Longrightarrow> bf.consistentS op = (bf (x::nat\<times>nat)) (bf\<^sub>T x)"
@@ -66,11 +76,11 @@ lemma bf_inductS':
   "\<lbrakk>\<And>j. bf.consistentS op = (bf (0, j)) (bf\<^sub>T (0, j));
     \<And>k j. \<lbrakk>K k k k;
            K j j j;
-           (rel_prod (K k) op = ===> bf.consistentS op =) bf bf\<^sub>T;
+           (rel_prod (K k) (eq_onp (\<lambda>x. x\<in>set [0..<n])) ===> bf.consistentS op =) bf bf\<^sub>T;
            (rel_prod (K k) (K j) ===> bf.consistentS op =) bf bf\<^sub>T
            \<rbrakk> \<Longrightarrow> bf.consistentS op = (bf (Suc k, j)) (bf\<^sub>T (Suc k, j))
    \<rbrakk> \<Longrightarrow> bf.consistentS op = (bf (x::nat\<times>nat)) (bf\<^sub>T x)"
-  unfolding K_def rel_prod.simps using bf_inductS by blast
+  unfolding K_def eq_onp_def rel_prod.simps using bf_inductS by blast
 
 lemma "bf.consistentDP bf\<^sub>T"
   by (dp_match induct: bf_inductS' simp: bf.simps simp\<^sub>T: bf\<^sub>T.simps)
