scratch/Scratch.thy
@@ -1,10 +1,76 @@
 theory Scratch
-  imports Main
+  imports "../DP_Consistency"
 begin
 term int
 term fold
   
-fun f :: "nat \<Rightarrow> nat" where
-  "f 0 = 0"
-| "f (Suc x) = fold op + (map (\<lambda>x. f) [0..<x]) 0"
-end
+context dp_consistency
+begin
+context
+  includes lifting_syntax
+begin
+term 0 (**)
+
+
+definition ceq :: "('a \<Rightarrow> 'a \<Rightarrow> bool) \<Rightarrow> ('param \<rightharpoonup> 'result, 'a) state \<Rightarrow> ('param \<rightharpoonup> 'result, 'a) state \<Rightarrow> bool" where
+  "ceq R s0 s1 \<equiv> (eq_onp consistentM ===> rel_prod R (eq_onp consistentM)) (runState s0) (runState s1)"
+  
+lemma ceq_intro:
+  fixes R s0 s1
+  assumes "\<And>M v0 M0 v1 M1. \<lbrakk>consistentM M; runState s0 M = (v0,M0); runState s1 M = (v1,M1)\<rbrakk> \<Longrightarrow> R v0 v1 \<and> M0=M1 \<and> consistentM M1"
+  shows "ceq R s0 s1"
+  unfolding ceq_def eq_onp_def rel_fun_def rel_prod_conv by (auto split: prod.split dest: assms)
+term 0 (**)
+
+lemma ceq_elim:
+  fixes R s0 s1
+  assumes "ceq R s0 s1" "consistentM M"
+  obtains v0 M0 v1 M1 where "runState s0 M = (v0, M0)" "runState s1 M = (v1, M1)" "R v0 v1" "M0=M1" "consistentM M1"
+  using assms unfolding ceq_def eq_onp_def rel_fun_def by (blast elim: rel_prod.cases)
+    
+term 0 (**)
+  
+lemma id\<^sub>T_cong:
+  fixes R x y
+  shows "(R ===> ceq R) return return"
+  unfolding rel_fun_def return_def by (fastforce intro: ceq_intro)
+thm id\<^sub>T_cong[THEN rel_funD]
+term 0 (**)
+  
+lemma bind_cong[transfer_rule]:
+  fixes R0 R1
+  shows "(ceq R0 ===> (R0 ===> ceq R1) ===> ceq R1) (op \<bind>) (op \<bind>)"
+  unfolding rel_fun_def bind_def by (fastforce intro!: ceq_intro elim!: ceq_elim)
+thm bind_cong[THEN rel_funD, THEN rel_funD]
+term 0 (**)
+
+lemma app\<^sub>T_cong[transfer_rule]:
+  shows "(ceq (R0 ===> ceq R1) ===> ceq R0 ===> ceq R1) (op .) (op .)"
+  unfolding fun_app_lifted_def by transfer_prover
+thm app\<^sub>T_cong[THEN rel_funD, THEN rel_funD]
+term 0 (**)
+  
+lemma map\<^sub>T_cong:
+  assumes "ceq R0 xs\<^sub>T ys\<^sub>T"
+  assumes "\<And>M. consistentM M \<Longrightarrow> case (runState f\<^sub>T M, runState g\<^sub>T M) of ((f, Mf), (g, Mg)) \<Rightarrow>
+            Mf = Mg \<and> consistentM Mg \<and> (case runState ys\<^sub>T Mg of (ys, Mys) \<Rightarrow> (\<forall>x\<in>set ys. ceq R1 (f x) (g x)))"
+  shows "ceq (list_all2 R1) (map\<^sub>T . f\<^sub>T . xs\<^sub>T) (map\<^sub>T . g\<^sub>T . ys\<^sub>T)"
+
+
+
+
+
+
+
+
+
+
+
+
+
+
+
+
+
+
+
